---
title: "Data Order Invariance"
author: "Dr. Dogucu"
output: 
  xaringan::moon_reader:
    css: slide-style.css
    nature:
      ratio: 16:9
      highlightStyle: github
      highlightLines: true
---

layout: true
  
<div class="my-header"></div>

<div class="my-footer"> From Bayes Rules! book
 Copyright &copy; Drs. Alicia Johnson, Miles Ott & Mine Dogucu. <a href="https://creativecommons.org/licenses/by-nc-sa/4.0/">CC BY-NC-SA 4.0</a></div> 

---

$$f(\theta | x_1,x_2) = f(\theta|x_2,x_1)$$

--

$$f(\theta|x_1) = \frac{\text{prior}\cdot \text{likelihood}}{\text{normalizing constant}} = \frac{f(\theta)L(\theta|x_1)}{f(x_1)}$$

--

$$f(\theta|x_2) = \frac{\text{prior}\cdot \text{likelihood}}{\text{normalizing constant}} = \frac{\frac{f(\theta)L(\theta|x_1)}{f(x_1)}L(\theta|x_2)}{f(x_2)}$$
--

$$f(\theta|x_1,x_2) =  \frac{f(\theta)L(\theta|x_1)L(\theta|x_2)}{f(x_1)f(x_2)}$$
--

$$f(\theta|x_2,x_1) =  \frac{f(\theta)L(\theta|x_2)L(\theta|x_1)}{f(x_2)f(x_1)}$$

--

$$f(\theta | x_1,x_2) = f(\theta|x_2,x_1)$$
